theories/heap_lang/adequacy.v
@@ -1,6 +1,7 @@
 From iris.program_logic Require Export weakestpre adequacy.
 From iris.algebra Require Import auth.
-From iris.heap_lang Require Import proofmode notation proph_map.
+From iris.heap_lang Require Import proofmode notation.
+From iris.base_logic.lib Require Import proph_map.
 From iris.proofmode Require Import tactics.
 Set Default Proof Using "Type".
 
